# Q1
## 1a
$$
\begin{cases}
x_0 = -1 \\
x_1 = 0 \\
x_2 = 1 \\
x_3 = 2
\end{cases}
,~
\begin{cases}
y_1 = 2 \\
y_2 = 7 \\
y_3 = 22 \\
y_4 = 71
\end{cases}
$$
We have 4 points, so we will construct a degree 3 polynomial $p(x) \in \mathcal{P}_3$ to interpolate the points.
$$
\begin{align}
p(-1) &= 2 \\
p(0) &= 7 \\
p(1) &= 22 \\
p(2) &= 71
\end{align}
\implies
\begin{bmatrix}
1 & -1 & 1 & -1 \\
1 & 0 & 0 & 0 \\
1 & 1 & 1 & 1 \\
1 & 2 & 4 & 8
\end{bmatrix}
\begin{bmatrix}
a_0 \\
a_1  \\
a_2 \\
a_3
\end{bmatrix}
= 
\begin{bmatrix}
2 \\
7 \\
22 \\
71
\end{bmatrix}
$$
Now use LU factorization to solve for $a_0, a_1, a_2, a_3$.
$$
A =
\begin{bmatrix}
1 & -1 & 1 & -1 \\
1 & 0 & 0 & 0 \\
1 & 1 & 1 & 1 \\
1 & 2 & 4 & 8
\end{bmatrix}
, ~
P_1 = I
, ~
P_1A = A,
L_1 =
\begin{bmatrix}
1 & 0 & 0 & 0 \\
-1 & 1 & 0 & 0 \\
-1 & 0 & 1 & 0 \\
-1 & 0 & 0 & 1
\end{bmatrix}
,~
L_1P_1A =
\begin{bmatrix}
1 & -1 & 1 & -1 \\
0 & 1 & -1 & 1 \\
0 & 2 & 0 & 2 \\
0 & 3 & 3 & 9
\end{bmatrix}
$$
$$
P_2 =
\begin{bmatrix}
1 & 0 & 0 & 0 \\
0 & 0 & 0 & 1 \\
0 & 0 & 1 & 0 \\
0 & 1 & 0 & 0
\end{bmatrix}
,~
P_2L_1P_1A =
\begin{bmatrix}
1 & -1 & 1 & -1 \\
0 & 3 & 3 & 9 \\
0 & 2 & 0 & 2 \\
0 & 1 & -1 & 1
\end{bmatrix}
,~
L_2 =
\begin{bmatrix}
1 & 0 & 0 & 0 \\
0 & 1 & 0 & 0 \\
0 & -\frac{2}{3} & 1 & 0 \\
0 & -\frac{1}{3} & 0 & 1
\end{bmatrix}
,~
L_2P_2L_1P_1A =
\begin{bmatrix}
1 & -1 & 1 & -1 \\
0 & 3 & 3 & 9 \\
0 & 0 & -2 & -4 \\
0 & 0 & -2 & -2
\end{bmatrix}
$$
$$
P_3 = I
,~
P_3L_2P_2L_1P_1A = \begin{bmatrix}
1 & -1 & 1 & -1 \\
0 & 3 & 3 & 9 \\
0 & 0 & -2 & -4 \\
0 & 0 & -2 & -2
\end{bmatrix}
,~
L_3 =
\begin{bmatrix}
1 & 0 & 0 & 0 \\
0 & 1 & 0 & 0 \\
0 & 0 & 1 & 0 \\
0 & 0 & -1 & 1
\end{bmatrix}
,~
L_3P_3L_2P_2L_1P_1A =
\begin{bmatrix}
1 & -1 & 1 & -1 \\
0 & 3 & 3 & 9 \\
0 & 0 & -2 & -4 \\
0 & 0 & 0 & 2
\end{bmatrix}
= U
$$
$$
P = P_3P_2P_1 = P_2 =
\begin{bmatrix}
1 & 0 & 0 & 0 \\
0 & 0 & 0 & 1 \\
0 & 0 & 1 & 0 \\
0 & 1 & 0 & 0
\end{bmatrix}
$$
$$
L_3P_3L_2P_2L_1P_1A = L_3\tilde{L}_2\tilde{L}_1P_3P_2P_1A
$$
$$
\begin{align}
\tilde{L}_2 &= P_3L_2P_3 = L_2 =
\begin{bmatrix}
1 & 0 & 0 & 0 \\
0 & 1 & 0 & 0 \\
0 & -\frac{2}{3} & 1 & 0 \\
0 & -\frac{1}{3} & 0 & 1
\end{bmatrix} \\
\tilde{L}_1 &= P_3P_2L_1P_2P_3 = P_2L_1P_2 =
\begin{bmatrix}
1 & 0 & 0 & 0 \\
-1 & 1 & 0 & 0 \\
-1 & 0 & 1 & 0 \\
-1 & 0 & 0 & 1
\end{bmatrix}
\end{align}
$$
$$
L = \tilde{L}_1^{-1} \tilde{L}_2^{-1} L_3^{-1} =
\begin{bmatrix}
1 & 0 & 0 & 0 \\
1 & 1 & 0 & 0 \\
1 & \frac{2}{3} & 1 & 0 \\
1 & \frac{1}{3} & 1 & 1
\end{bmatrix}
$$
$PA = LU \implies LUx = Pb \implies Ld = Pb, Ux = d$
$$
Pb =
\begin{bmatrix}
2 \\
71 \\
22 \\
7
\end{bmatrix}
\implies
\begin{bmatrix}
1 & 0 & 0 & 0 \\
1 & 1 & 0 & 0 \\
1 & \frac{2}{3} & 1 & 0 \\
1 & \frac{1}{3} & 1 & 1
\end{bmatrix}
\begin{bmatrix}
d_0 \\
d_1 \\
d_2 \\
d_3
\end{bmatrix}
=
\begin{bmatrix}
2 \\
71 \\
22 \\
7
\end{bmatrix}
$$
$$
\begin{cases}
d_0 = 2 \\
d_1 = 69 \\
d_2 = -26 \\
d_3 = 8
\end{cases}
$$
$$
Ux = d \implies
\begin{bmatrix}
1 & -1 & 1 & -1 \\
0 & 3 & 3 & 9 \\
0 & 0 & -2 & -4 \\
0 & 0 & 0 & 2
\end{bmatrix}
\begin{bmatrix}
a_0 \\
a_1 \\
a_2 \\
a_3
\end{bmatrix}
=
\begin{bmatrix}
2 \\
69 \\
-26 \\
8
\end{bmatrix}
$$
$$
\begin{cases}
a_3 = 4 \\
a_2 = 5 \\
a_1 = 6 \\
a_0 = 7
\end{cases}
$$
Therefore our interpolation polynomial in monomial basis form is $p(x) = 7 + 6x + 5x^2 + 4x^3$.
## 1b
For Lagrange basis form our interpolation polynomial is: $p(x) = \displaystyle \sum_{i = 0}^{n} \ell_i(x) y_i$
$$
\begin{align}
\ell_0(x) &= \frac{x - x_1}{x_0 - x_1} \cdot \frac{x - x_2}{x_0 - x_2} \cdot \frac{x - x_3}{x_0 - x_3} = \frac{x}{-1} \cdot \frac{x - 1}{-1 - 1} \cdot \frac{x - 2}{-1 - 2} = -\frac{1}{6}x(x-1)(x-2) \\
\ell_1(x) &= \frac{x - x_0}{x_1 - x_0} \cdot \frac{x - x_2}{x_1 - x_2} \cdot \frac{x - x_3}{x_1 - x_3} = \frac{x + 1}{1} \cdot \frac{x - 1}{-1} \cdot \frac{x - 2}{-2} = \frac{1}{2}(x+1)(x-1)(x-2) \\
\ell_2(x) &= \frac{x - x_0}{x_2 - x_0} \cdot \frac{x - x_1}{x_2 - x_1} \cdot \frac{x - x_3}{x_2 - x_3} = \frac{x + 1}{2} \cdot \frac{x}{1} \cdot \frac{x - 2}{-1} = -\frac{1}{2}x(x+1)(x-2) \\
\ell_3(x) &= \frac{x - x_0}{x_3 - x_0} \cdot \frac{x - x_1}{x_3 - x_1} \cdot \frac{x - x_2}{x_3 - x_2} = \frac{x + 1}{3} \cdot \frac{x}{2} \cdot \frac{x - 1}{1} = \frac{1}{6}x(x+1)(x-1)
\end{align}
$$
Lagrange basis form is:
$$
p(x) = -\frac{2}{6}x(x-1)(x-2) + \frac{7}{2}(x+1)(x-1)(x-2) - \frac{22}{2}x(x+1)(x-2) + \frac{71}{6}x(x+1)(x-1)
$$
To confirm it is the same polynomial as in monomial basis form, we expand all terms:
$$
\begin{align}
p(x) &= \left( -\frac{1}{3}x^3 + x^2 - \frac{2}{3}x \right) + \left( \frac{7}{2}x^3 - 7x^2 - \frac{7}{2} x + 7 \right) - (11x^3 - 11x^2 - 22x) + \left( \frac{71}{6}x^3 - \frac{71}{6}x \right) \\
&= \left( -\frac{2}{6} + \frac{21}{6} - 11 + \frac{71}{6} \right)x^3 + (1 - 7 + 11)x^2 + \left( -\frac{4}{6} - \frac{21}{6} + 22 - \frac{71}{6} \right)x + 7 \\
&= 4x^3 + 5x^2 + 6x + 7
\end{align}
$$
## 1c
$$
\begin{align}
p(x) &= y[x_0] + (x - x_0)y[x_1, x_0] + (x - x_0)(x - x_1)y[x_2, x_1, x_0] + (x - x_0)(x - x_1)(x - x_2)y[x_3, x_2, x_1, x_0]
\end{align}
$$

| $x$ | $y[x_i]$ | $y[x_{i+1}, x_i]$ | $y[x_{i+2}, x_{i+1}, x_i]$ | $y[x_{i+3}, x_{i+2}, x_{i+1}, x_i]$ |
|-|-|-|-|-|
|-1|2||||
|||$\frac{7-2}{0-(-1)}=5$|||
|0|7||$\frac{15-5}{1-(-1)}=5$||
|||$\frac{22-7}{1-0}=15$||$\frac{17-5}{2-(-1)}=4$|
|1|22||$\frac{49-15}{2-0}=17$||
|||$\frac{71-22}{2-1}=49$|||
|2|71||||
Newton basis form of polynomial interpolant:
$$
\begin{align}
p(x) &= 2 + 5(x - x_0) + 5(x - x_0)(x - x_1) + 4(x - x_0)(x - x_1)(x - x_2) \\
&= 2 + 5(x + 1) + 5x(x + 1) + 4x(x + 1)(x - 1)
\end{align}
$$
To confirm it is the same polynomial as in monomial basis form, we expand all terms:
$$
\begin{align}
p(x) &= 2 + (5x + 5) + (5x^2 + 5x) + (4x^3 - 4x) \\
&= 7 + 6x + 5x^2 + 4x^3
\end{align}
$$
## 1d
We can get the individual linear equations using $y = \frac{y_a - y_b}{x_a - x_b}x + b$ and looking at each pair of adjacent points.
Line between $(-1, 2)$ and $(0, 7)$: $y = 5x + 7$
Line between $(0, 7)$ and $(1, 22)$: $y = 15x + 7$
Line between $(1, 22)$ and $(2, 71)$: $y = 49x - 27$
Thus our interpolating linear spline is:
$$
p(x) =
\begin{cases}
5x + 7 & \text{if } -1 \le x \le 0 \\
15x + 7 & \text{if } 0 \le x \le 1 \\
49x - 27 & \text{if } 1 \le x \le 2
\end{cases}
$$
## 1e
To evaluate the linear spline at any $x \in \mathbb{R}$, we need to:
1. Find the interval of the spline in which $x$ lies in
2. Evaluate $x$ with the corresponding linear equation for the interval
For step 1, if the given data points are in sorted order, we are able to use binary search to get the interval in $O(\log n)$ time instead of $O(n)$ time.

The main disadvantage of this spline over the polynomial interpolant is that the spline is not $C_1$ continuous and thus may not be able to extract derivative information at all points (in particular the piece-wise transition points).

The main advantage is the speed and simplicity in computing the spline over the polynomial. It is clearly much quicker to compute $n-1$ linear equations going through only $2$ points rather than going through the different processes presented in parts a, b, or c. 
Additionally, it has the benefit of being able to mitigate the Runge Phenomenon.
# Q2

## 2a
monomial basis spans $\mathcal{P}_n$ and linearly independent
$x_i$ distinct

Since the monomial basis is linearly independent, for any $x$:
$$
a_0 + a_1x + a_2x^2 + \cdots + a_nx^n = 0 \iff a_0 = a_1 = \cdots = a_n = 0
$$

Let the $i^{th}$ column of the Vandermonde matrix be denoted $v_i$. A matrix is nonsingular/invertible iff its columns are linearly independent or alternatively that no column is a linear combination of the other columns. That is for scalars $a_0, a_1, \cdots, a_n \in \mathbb{R}$, we have that $a_0v_0 + a_1v_1 + \cdots + a_nv_n = 0 \iff a_0 = a_1 = \cdots = a_n = 0$.
$$
V =
\begin{bmatrix}
1 & x_0^1 & x_0^2 & \cdots & x_0^n \\
1 & x_1^1 & x_1^2 & \cdots & x_1^n \\
\vdots \\
1 & x_n^1 & x_n^2 & \cdots & x_n^n
\end{bmatrix}
=
\begin{bmatrix}
v_0 & v_1 & v_2 & \cdots & v_n
\end{bmatrix}
$$
Notice that for  $i \ne j, x^i \ne ax^j, \forall a \in \mathbb{R}$. 

## 2b

# Q3
$$
\ell_i(x_j) =
\begin{cases}
1 & \text{if } j = i  \\
0 & \text{if } j \ne i \\
\end{cases}
\implies
q(x_j) = \sum_{i = 0}^{n} \ell_i(x_j) = 1, \forall j = 0, \cdots, n
$$
If we define $f(x) = q(x) - 1$.
$$
f(x_j) = q(x_j) - 1 = 0, \forall j = 0, \cdots, n
$$
Thus $f(x)$ has $n+1$ roots (since $x_j$ are distinct).
However, $\ell_i(x) \in \mathcal{P}_n \implies q(x) \in \mathcal{P}_n \implies f(x) \in \mathcal{P}_n$ thus $f(x)$ is (at most) an $n$-degree polynomial, which by the Fundamental Theorem of Algebra has at most $n$ distinct roots. As $f(x)$ has $n+1$ roots, it must be that $f(x) = 0, \forall x \in \mathbb{R} \implies q(x) = 1, \forall x \in \mathbb{R}$ as wanted.
# Q4
## 4a
Note that we already have the values for $a_0, a_1, \cdots, a_n$.
With the monomial basis, our interpolating polynomial will have the form:
$$
\begin{align}
p(x) &= a_0 + a_1x + a_2x^2 + \cdots + a_nx^n \\
&= a_0 + x(a_1 + a_2x + a_3x^2 + \cdots + a_n x^{n-1}) \\
&= a_0 + x(a_1 + x(a_2 + a_3x + \cdots + a_n x^{n-2})) \\
&~~\vdots \\
&= a_0 + x(a_1 + x(a_2 + x(a_3 +x(\cdots + x(a_{n-1} + xa_n))))
\end{align}
$$
**Pseudocode:**
$out := a_n$
for $i := n-1$ to $0$ do
	$out := out \times x + a_i$

Writing it as such, we are able to evaluate the polynomial in linear $O(n)$ flops.
## 4b
Note that we have the values for $a_0, a_1, \cdots, a_n$ as well as $x_0, x_1, \cdots, x_n$
With the divided-difference basis, our interpolating polynomial will have the form:
$$
\begin{align}
p(x) &= a_0 + a_1(x - x_0) + a_2(x-x_0)(x-x_1) + \cdots + a_n(x-x_0)(x-x_1)\cdots(x-x_{n-1}) \\
&= a_0 + (x - x_0) \left( a_1 + a_2(x-x_1) + \cdots + a_n(x-x_1)\cdots(x-x_{n-1}) \right) \\
&= a_0 + (x-x_0)(a_1 + (x-x_1)(a_2 + \cdots + a_n(x-x_2)\cdots(x-x_{n-1}))) \\
&~~\vdots \\
&= a_0 + (x-x_0)(a_1+(x-x_1)(a_2 + (x-x_2)(\cdots (a_{n-1} + (x-x_{n-1})(a_n))))
\end{align}
$$
**Pseudocode:**
$out := a_n$
for $i := n-1$ to $0$ do
	$out := out \times (x - x_i) + a_i$

Similar to part a with the monomial basis, we are able to evaluate the polynomial in $O(n)$ flops.